examples/arm6/onestepScript.sml
@@ -1,4 +1,4 @@
-(* app load ["bossLib","combinTheory","arithmeticTheory","prim_recTheory"]; *)
+(* app load ["combinTheory","arithmeticTheory","prim_recTheory"]; *)
 open HolKernel boolLib Q Parse bossLib simpLib numLib
      combinTheory arithmeticTheory prim_recTheory;
 
@@ -7,178 +7,6 @@ open HolKernel boolLib Q Parse bossLib simpLib numLib
 val _ = new_theory "onestep";
 
 (* --------------------------------------------------------*)
-(* - Iterated Maps ----------------------------------------*)
-(* --------------------------------------------------------*)
-
-val IMAP_def = Define `
-  IMAP G init next =
-    (!a. (G 0 a = init a)) /\
-    (!t a. (G (SUC t) a = next (G t a)))`;
-
-(* --------------------------------------------------------*)
-(* - Data Abstraction Criterion ---------------------------*)
-(* --------------------------------------------------------*)
-
-val ONTO_INIT_def = Define `
-  ONTO_INIT psi init init' =
-    !a. ?b. psi (init' b) = init a`;
-
-(* --------------------------------------------------------*)
-(* - Immersions : General, Uniform and Adjunct ------------*)
-(* --------------------------------------------------------*)
-
-val IMM_def = Define `
-  IMM imm =
-    ((!a. imm a 0 = 0) /\
-     (!a t1 t2. t1 < t2 ==> imm a t1 < imm a t2))`;
-
-val UIMM_def = Define `
-  UIMM imm G dur =
-    ((!a. 0 < dur a) /\
-     (!a. imm a 0 = 0) /\
-     (!a t. imm a (SUC t) = dur (G (imm a t) a) + imm a t))`;
-
-val AUIMM_def = Define `
-  AUIMM imm1 imm2 G dur1 dur2 =
-    ((UIMM imm2 G dur2) /\
-     (!a. 0 < dur1 a) /\
-     (!a. imm1 a 0 = 0) /\
-     (!a t. imm1 a (SUC t) = dur1 (G (imm2 a t) a) + imm1 a t))`;
-
-(* --------------------------------------------------------*)
-(* - Correctness Definitions ------------------------------*)
-(* --------------------------------------------------------*)
-
-val CORRECT_def = Define `
-  CORRECT spec impl imm psi =
-    IMM imm /\ ONTO_INIT psi (spec 0) (impl 0) /\
-    (!t a. spec t (psi a) = psi (impl (imm a t) a))`;
-
-val CORRECT_SUP_def = Define `
-  CORRECT_SUP spec impl imm1 imm2 psi =
-    IMM imm1 /\ IMM imm2 /\ ONTO_INIT psi (spec 0) (impl 0) /\
-    (!r a. spec (imm1 a r) (psi a) = psi (impl (imm2 a r) a))`;
-
-(* --------------------------------------------------------*)
-(* - Time-Consistent State Functions ----------------------*)
-(* --------------------------------------------------------*)
-
-val TCON_def = Define `
-  TCON G = !t1 t2 a. G (t1 + t2) a = G t1 (G t2 a)`;
-
-val TCON_IMM_def = Define `
-  TCON_IMM G imm =
-    !t1 t2 a.
-      G (imm (G (imm a t2) a) t1 + imm a t2) a =
-      G (imm (G (imm a t2) a) t1) (G (imm a t2) a)`;
-
-(* --------------------------------------------------------*)
-(* - Uniform Immersions are Immersions --------------------*)
-(* --------------------------------------------------------*)
-
-val SUC_COMM_LEMMA = prove(
-  `!t p. t + (SUC p + 1) = SUC (t + (p + 1))`,
-  RW_TAC arith_ss []
-);
-
-val UIMM_MONO_LEMMA = prove(
-  `!imm G dur a t. UIMM imm G dur ==> imm a t < imm a (SUC t)`,
-  RW_TAC std_ss [UIMM_def,ADD_COMM,LESS_NOT_EQ,LESS_ADD_NONZERO]
-);
-
-val UIMM_MONO_LEMMA2 = prove(
-  `!imm G dur a t p. UIMM imm G dur ==> imm a t < imm a (t + (p + 1))`,
-  REPEAT STRIP_TAC
-   THEN IMP_RES_TAC UIMM_MONO_LEMMA
-   THEN Induct_on `p`
-   THENL [
-     ASM_SIMP_TAC std_ss [SYM (num_CONV ``1``),GSYM ADD1,UIMM_MONO_LEMMA],
-     FULL_SIMP_TAC std_ss  [SUC_COMM_LEMMA,LESS_IMP_LESS_ADD,ADD_COMM,UIMM_def]
-   ]
-);
-
-val UIMM_IS_IMM_LEMMA = store_thm("UIMM_IS_IMM_LEMMA",
-  `!imm G dur. UIMM imm G dur ==> IMM imm`,
-  REPEAT STRIP_TAC
-    THEN IMP_RES_TAC UIMM_MONO_LEMMA2
-    THEN FULL_SIMP_TAC std_ss [UIMM_def]
-    THEN RW_TAC std_ss [IMM_def]
-    THEN IMP_RES_TAC LESS_ADD_1
-    THEN ASM_SIMP_TAC std_ss [UIMM_MONO_LEMMA2]
-);
-
-(* --------------------------------------------------------*)
-(* - Uniform Adjunct Immersions are Immersions ------------*)
-(* --------------------------------------------------------*)
-
-
-val AUIMM_MONO_LEMMA = prove(
-  `!G imm1 imm2 dur1 dur2 a t. AUIMM imm1 imm2 G dur1 dur2 ==>
-                               imm1 a t < imm1 a (SUC t)`,
-  RW_TAC std_ss [AUIMM_def,ADD_COMM,LESS_NOT_EQ,LESS_ADD_NONZERO]
-);
-
-val AUIMM_MONO_LEMMA2 = prove(
-  `!G imm1 imm2 dur1 dur2 a t p. AUIMM imm1 imm2 G dur1 dur2 ==>
-                                 imm1 a t < imm1 a (t + (p + 1))`,
-  REPEAT STRIP_TAC
-   THEN IMP_RES_TAC AUIMM_MONO_LEMMA
-   THEN Induct_on `p` THENL [
-     ASM_SIMP_TAC std_ss [SYM (num_CONV ``1``),GSYM ADD1,AUIMM_MONO_LEMMA],
-     FULL_SIMP_TAC std_ss [SUC_COMM_LEMMA,LESS_IMP_LESS_ADD,ADD_COMM,AUIMM_def]
-  ]
-);
-
-val AUIMM_IS_IMM_LEMMA = store_thm("AUIMM_IS_IMM_LEMMA",
-  `!G imm1 imm2 dur1 dur2. AUIMM imm1 imm2 G dur1 dur2 ==> (IMM imm1 /\ IMM imm2)`,
-  REPEAT STRIP_TAC
-    THEN IMP_RES_TAC AUIMM_MONO_LEMMA2
-    THEN FULL_SIMP_TAC std_ss [AUIMM_def]
-    THEN IMP_RES_TAC UIMM_IS_IMM_LEMMA
-    THEN RW_TAC std_ss [IMM_def]
-    THEN IMP_RES_TAC LESS_ADD_1
-    THEN ASM_SIMP_TAC std_ss [AUIMM_MONO_LEMMA2]
-);
-
-(* --------------------------------------------------------*)
-(* - Time-Consistency Results -----------------------------*)
-(* --------------------------------------------------------*)
-
-val TC_IMP_IMAP = store_thm("TC_IMP_IMAP",
-  `!G. TCON G ==> ?init next. IMAP G init next`,
-  RW_TAC std_ss [TCON_def,IMAP_def]
-    THEN EXISTS_TAC `G 0`
-    THEN EXISTS_TAC `G (SUC 0)`
-    THEN POP_ASSUM (fn th => ASSUME_TAC (GEN_ALL (ONCE_REWRITE_RULE [ADD_COMM] (SPECL [`1`,`t`] th))))
-    THEN ASM_SIMP_TAC std_ss [ADD1,SYM ONE]
-);
-
-val TC_LEMMA = store_thm("TC_LEMMA",
-  `!G init next. IMAP G init next ==> (TCON G = (!t a. init (G t a) = G t a))`,
-  RW_TAC std_ss [TCON_def,IMAP_def]
-    THEN EQ_TAC
-    THEN REPEAT STRIP_TAC
-    THENL [
-       POP_ASSUM (fn th => GEN_REWRITE_TAC (ONCE_DEPTH_CONV o RAND_CONV) empty_rewrites
-                                           [(REDUCE_RULE (SPECL [`0`,`t`] th))])
-         THEN ASM_REWRITE_TAC [],
-     Induct_on `t1`
-       THEN ASM_SIMP_TAC std_ss [ADD_CLAUSES]
-    ]
-);
-
-val TC_I_LEMMA = store_thm("TC_I_LEMMA",
-  `!G next. IMAP G I next ==> TCON G`,
-  REPEAT STRIP_TAC
-    THEN IMP_RES_TAC TC_LEMMA
-    THEN ASM_SIMP_TAC std_ss [I_THM]
-);
-
-val TC_IMP_TC_IMM = store_thm("TC_IMP_TC_IMM",
-  `!G. TCON G ==> !Imm. TCON_IMM G Imm`,
-  RW_TAC std_ss [TCON_def,TCON_IMM_def]
-);
-  
 val FUNPOW_THM = store_thm("FUNPOW_THM",
   `!f n x. FUNPOW f n (f x) = f (FUNPOW f n x)`,
   Induct_on `n` THEN ASM_REWRITE_TAC [FUNPOW]
@@ -186,7 +14,7 @@ val FUNPOW_THM = store_thm("FUNPOW_THM",
 
 val FUNPOW_THM2 = store_thm("FUNPOW_THM2",
   `!f n x. FUNPOW f (SUC n) x = f (FUNPOW f n x)`,
-  Induct_on `n` THEN RW_TAC std_ss [FUNPOW,FUNPOW_THM]
+  Induct_on `n` THEN RW_TAC bool_ss [FUNPOW,FUNPOW_THM]
 );
 
 val FUNPOW_EVAL = store_thm("FUNPOW_EVAL",
@@ -198,241 +26,391 @@ val FUNPOW_COMP_LEMMA = prove(
   `!f a b x. FUNPOW f (a+b) x = FUNPOW f a (FUNPOW f b x)`,
   Induct_on `b` THEN ASM_REWRITE_TAC [ADD_CLAUSES,FUNPOW]
 );
+(* --------------------------------------------------------*)
+
+(*--------------------------------------------------------
+  - Iterated Maps ----------------------------------------
+  --------------------------------------------------------*)
+
+val IMAP_def = Define `
+  IMAP f init next =
+    (!a. (f 0 a = init a)) /\
+    (!t a. (f (SUC t) a = next (f t a)))`;
+
+val IS_IMAP_def = Define`
+  IS_IMAP f = ?init next. IMAP f init next`;
+
+(*--------------------------------------------------------
+  - Data Abstraction Criterion ---------------------------
+  --------------------------------------------------------*)
+
+val DATA_ABSTRACTION_def = Define `
+  DATA_ABSTRACTION abs init init' =
+    !a. ?b. abs (init' b) = init a`;
+
+(*--------------------------------------------------------
+  - Immersions : General, Uniform and Adjunct ------------
+  --------------------------------------------------------*)
+
+val IMMERSION_def = Define `
+  IMMERSION imm =
+    ((!a. imm a 0 = 0) /\
+     (!a t1 t2. t1 < t2 ==> imm a t1 < imm a t2))`;
+
+val UIMMERSION_def = Define `
+  UIMMERSION imm f dur =
+    ((!a. 0 < dur a) /\
+     (!a. imm a 0 = 0) /\
+     (!a t. imm a (SUC t) = dur (f (imm a t) a) + imm a t))`;
+
+val AUIMMERSION_def = Define `
+  AUIMMERSION imm1 imm2 f dur1 dur2 =
+    ((UIMMERSION imm2 f dur2) /\
+     (!a. 0 < dur1 a) /\
+     (!a. imm1 a 0 = 0) /\
+     (!a t. imm1 a (SUC t) = dur1 (f (imm2 a t) a) + imm1 a t))`;
+
+val UNIFORM_def = Define`
+  UNIFORM imm f = ?dur. UIMMERSION imm f dur`;
+
+val ADJUNCT_def = Define`
+  ADJUNCT imm1 imm2 f = ?dur1 dur2. AUIMMERSION imm1 imm2 f dur1 dur2`;
+
+(*--------------------------------------------------------
+  - Correctness Definitions ------------------------------
+  --------------------------------------------------------*)
+
+val CORRECT_def = Define `
+  CORRECT spec impl imm abs =
+    IMMERSION imm /\ DATA_ABSTRACTION abs (spec 0) (impl 0) /\
+    (!t a. spec t (abs a) = abs (impl (imm a t) a))`;
+
+val CORRECT_SUP_def = Define `
+  CORRECT_SUP spec impl imm1 imm2 abs =
+    IMMERSION imm1 /\ IMMERSION imm2 /\ DATA_ABSTRACTION abs (spec 0) (impl 0) /\
+    (!r a. spec (imm1 a r) (abs a) = abs (impl (imm2 a r) a))`;
+
+val IS_CORRECT_def = Define`
+  IS_CORRECT spec impl = ?imm abs. CORRECT spec impl imm abs`;
+
+val IS_CORRECT_SUP_def = Define`
+  IS_CORRECT_SUP spec impl = ?imm1 imm2 abs. CORRECT_SUP spec impl imm1 imm2 abs`;
+ 
+(*--------------------------------------------------------
+  - Time-Consistent State Functions ----------------------
+  --------------------------------------------------------*)
+
+val TCON_def = Define `
+  TCON f = !t1 t2 a. f (t1 + t2) a = f t1 (f t2 a)`;
+
+val TCON_IMMERSION_def = Define `
+  TCON_IMMERSION f imm =
+    !t1 t2 a.
+      f (imm (f (imm a t2) a) t1 + imm a t2) a =
+      f (imm (f (imm a t2) a) t1) (f (imm a t2) a)`;
+
+(*--------------------------------------------------------
+  - Uniform Immersions are Immersions --------------------
+  --------------------------------------------------------*)
+
+val SUC_COMM_LEMMA = prove(
+  `!t p. t + (SUC p + 1) = SUC (t + (p + 1))`,
+  ARITH_TAC
+);
+
+val UIMMERSION_MONO_LEMMA = prove(
+  `!imm f dur a t. UIMMERSION imm f dur ==> imm a t < imm a (SUC t)`,
+  RW_TAC bool_ss [UIMMERSION_def,ADD_COMM,LESS_NOT_EQ,LESS_ADD_NONZERO]
+);
+
+val UIMMERSION_MONO_LEMMA2 = prove(
+  `!imm f dur a t p. UIMMERSION imm f dur ==> imm a t < imm a (t + (p + 1))`,
+  REPEAT STRIP_TAC
+   THEN IMP_RES_TAC UIMMERSION_MONO_LEMMA
+   THEN Induct_on `p`
+   THENL [
+     ASM_REWRITE_TAC [SYM ONE,GSYM ADD1,UIMMERSION_MONO_LEMMA],
+     FULL_SIMP_TAC bool_ss  [SUC_COMM_LEMMA,LESS_IMP_LESS_ADD,ADD_COMM,UIMMERSION_def]
+   ]
+);
+
+val UIMMERSION_IS_IMMERSION_LEMMA = store_thm("UIMMERSION_IS_IMMERSION_LEMMA",
+  `!imm f dur. UIMMERSION imm f dur ==> IMMERSION imm`,
+  REPEAT STRIP_TAC
+    THEN IMP_RES_TAC UIMMERSION_MONO_LEMMA2
+    THEN FULL_SIMP_TAC bool_ss [UIMMERSION_def]
+    THEN RW_TAC bool_ss [IMMERSION_def]
+    THEN IMP_RES_TAC LESS_ADD_1
+    THEN ASM_REWRITE_TAC [UIMMERSION_MONO_LEMMA2]
+);
+
+val UNIFORM_IMP_IMMERSION = store_thm("UNIFORM_IMP_IMMERSION",
+  `!imm f. UNIFORM imm f ==> IMMERSION imm`,
+  PROVE_TAC [UNIFORM_def,UIMMERSION_IS_IMMERSION_LEMMA]
+);
+
+(*--------------------------------------------------------
+  - Uniform Adjunct Immersions are Immersions ------------
+  --------------------------------------------------------*)
+
+val AUIMMERSION_MONO_LEMMA = prove(
+  `!f imm1 imm2 dur1 dur2 a t.
+     AUIMMERSION imm1 imm2 f dur1 dur2 ==> imm1 a t < imm1 a (SUC t)`,
+  RW_TAC bool_ss [AUIMMERSION_def,ADD_COMM,LESS_NOT_EQ,LESS_ADD_NONZERO]
+);
+
+val AUIMMERSION_MONO_LEMMA2 = prove(
+  `!f imm1 imm2 dur1 dur2 a t p.
+     AUIMMERSION imm1 imm2 f dur1 dur2 ==>imm1 a t < imm1 a (t + (p + 1))`,
+  REPEAT STRIP_TAC
+   THEN IMP_RES_TAC AUIMMERSION_MONO_LEMMA
+   THEN Induct_on `p` THENL [
+     ASM_REWRITE_TAC [SYM ONE,GSYM ADD1,AUIMMERSION_MONO_LEMMA],
+     FULL_SIMP_TAC bool_ss [SUC_COMM_LEMMA,LESS_IMP_LESS_ADD,ADD_COMM,AUIMMERSION_def]
+  ]
+);
+
+val AUIMMERSION_IS_IMMERSION_LEMMA = store_thm("AUIMMERSION_IS_IMMERSION_LEMMA",
+  `!f imm1 imm2 dur1 dur2.
+      AUIMMERSION imm1 imm2 f dur1 dur2 ==> IMMERSION imm1 /\ IMMERSION imm2`,
+  REPEAT STRIP_TAC
+    THEN IMP_RES_TAC AUIMMERSION_MONO_LEMMA2
+    THEN FULL_SIMP_TAC bool_ss [AUIMMERSION_def]
+    THEN IMP_RES_TAC UIMMERSION_IS_IMMERSION_LEMMA
+    THEN RW_TAC bool_ss [IMMERSION_def]
+    THEN IMP_RES_TAC LESS_ADD_1
+    THEN ASM_REWRITE_TAC [AUIMMERSION_MONO_LEMMA2]
+);
+
+val ADJUNCT_IMP_IMMERSIONS = store_thm("ADJUNCT_IMP_IMMERSIONS",
+  `!imm1 imm2 f. ADJUNCT imm1 imm2 f ==> IMMERSION imm1 /\ IMMERSION imm2`,
+  PROVE_TAC [ADJUNCT_def,AUIMMERSION_IS_IMMERSION_LEMMA]
+);
+
+(*--------------------------------------------------------
+  - Correct then Super Correct ---------------------------
+  --------------------------------------------------------*)
+
+val CORRECT_IMP_CORRECT_SUP = store_thm("CORRECT_IMP_CORRECT_SUP",
+  `!spec impl. IS_CORRECT spec impl ==> IS_CORRECT_SUP spec impl`,
+  RW_TAC bool_ss [IS_CORRECT_def,IS_CORRECT_SUP_def]
+    THEN EXISTS_TAC `\a t. t`
+    THEN EXISTS_TAC `imm`
+    THEN EXISTS_TAC `abs`
+    THEN FULL_SIMP_TAC arith_ss [CORRECT_def,CORRECT_SUP_def,IMMERSION_def]
+);
+
+(*--------------------------------------------------------
+  - Time-Consistency Results -----------------------------
+  --------------------------------------------------------*)
+
+val TC_IMP_IMAP = store_thm("TC_IMP_IMAP",
+  `!f. TCON f ==> IS_IMAP f`,
+  RW_TAC bool_ss [TCON_def,IMAP_def,IS_IMAP_def]
+    THEN EXISTS_TAC `f 0`
+    THEN EXISTS_TAC `f (SUC 0)`
+    THEN POP_ASSUM (fn th => ASSUME_TAC (GEN_ALL (ONCE_REWRITE_RULE [ADD_COMM] (SPECL [`1`,`t`] th))))
+    THEN ASM_REWRITE_TAC [ADD1,SYM ONE]
+);
+
+val TC_THM = store_thm("TC_THM",
+  `!f. TCON f = IS_IMAP f /\ (!t a. f 0 (f t a) = f t a)`,
+  STRIP_TAC THEN EQ_TAC
+    THEN REPEAT STRIP_TAC
+    THENL [
+      PROVE_TAC [TC_IMP_IMAP],
+      FULL_SIMP_TAC bool_ss [TCON_def]
+        THEN POP_ASSUM (fn th => REWRITE_TAC [GSYM (REDUCE_RULE (SPECL [`0`,`t`] th))]),
+      FULL_SIMP_TAC bool_ss [TCON_def,IS_IMAP_def,IMAP_def]
+        THEN Induct_on `t1` THEN ASM_REWRITE_TAC [ADD_CLAUSES]
+    ]
+);
+
+val TC_I_LEMMA = store_thm("TC_I_LEMMA",
+  `!f next. IMAP f I next ==> TCON f`,
+  PROVE_TAC [TC_THM,IS_IMAP_def,IMAP_def,I_THM]
+);
+
+val TC_IMP_TC_IMMERSION = store_thm("TC_IMP_TC_IMMERSION",
+  `!f. TCON f ==> !imm. TCON_IMMERSION f imm`,
+  RW_TAC bool_ss [TCON_def,TCON_IMMERSION_def]
+);
+
+val IMAP_INIT = store_thm("IMAP_INIT",
+  `!f init next. IMAP f init next ==> (f 0 = init)`,
+   RW_TAC bool_ss [IMAP_def,FUN_EQ_THM]
+);
 
 val STATE_FUNPOW_LEMMA = store_thm("STATE_FUNPOW_LEMMA",
-  `!G init next t a. IMAP G init next ==> (G t a = FUNPOW next t (init a))`,
+  `!f init next. IMAP f init next ==> (!t a. f t a = FUNPOW next t (init a))`,
   REWRITE_TAC [IMAP_def]
    THEN REPEAT STRIP_TAC
    THEN Induct_on `t`
    THEN ASM_REWRITE_TAC [FUNPOW,FUNPOW_THM]
 );
 
-val TC_IMM_LEMMA = store_thm("TC_IMM_LEMMA",
-  `!G init next imm. (IMM imm /\ (IMAP G init next)) ==>
-     (TCON_IMM G imm = (!t a. init (G (imm a t) a) = G (imm a t) a))`,
-  RW_TAC std_ss [IMM_def,TCON_IMM_def]
+val STATE_FUNPOW_LEMMA2 = store_thm("STATE_FUNPOW_LEMMA2",
+  `!f init next. IMAP f init next ==> (!t a. f t a = FUNPOW next t (f 0 a))`,
+  PROVE_TAC [IMAP_INIT,STATE_FUNPOW_LEMMA]
+);
+
+val TC_IMMERSION_LEMMA = store_thm("TC_IMMERSION_LEMMA",
+  `!f imm. IMMERSION imm /\ TCON_IMMERSION f imm ==> (!t a. f 0 (f (imm a t) a) = f (imm a t) a)`,
+  RW_TAC bool_ss [TCON_IMMERSION_def,IMMERSION_def]
+    THEN POP_ASSUM (fn th => ASSUME_TAC (SPECL [`0`,`t`,`a`] th))
+    THEN PAT_ASSUM `!a. imm a 0 = 0` (fn th => RULE_ASSUM_TAC (SIMP_RULE arith_ss [th]))
+    THEN POP_ASSUM (fn th => REWRITE_TAC [SYM th])
+);
+
+val TC_IMMERSION_LEMMA2 = store_thm("TC_IMMERSION_LEMMA2",
+  `!f imm. IMMERSION imm /\ IS_IMAP f ==>
+     (TCON_IMMERSION f imm = !t a. f 0 (f (imm a t) a) = f (imm a t) a)`,
+  RW_TAC bool_ss [IS_IMAP_def,IMMERSION_def,TCON_IMMERSION_def]
    THEN EQ_TAC
    THEN REPEAT STRIP_TAC THENL [
-     RULE_ASSUM_TAC (REWRITE_RULE [IMAP_def])
-       THEN POP_ASSUM (fn th => ASSUME_TAC (SPECL [`0`,`t`] th))
+     POP_ASSUM (fn th => ASSUME_TAC (SPECL [`0`,`t`] th))
        THEN PAT_ASSUM `!a. imm a 0 = 0` (fn th => RULE_ASSUM_TAC (SIMP_RULE arith_ss [th]))
-       THEN POP_ASSUM (fn th => GEN_REWRITE_TAC (ONCE_DEPTH_CONV o RAND_CONV) empty_rewrites [th])
-       THEN ASM_SIMP_TAC std_ss [],
-     IMP_RES_TAC STATE_FUNPOW_LEMMA
+       THEN PROVE_TAC [],
+     IMP_RES_TAC IMAP_INIT
+       THEN POP_ASSUM (fn th => RULE_ASSUM_TAC (REWRITE_RULE [th]))
+       THEN IMP_RES_TAC STATE_FUNPOW_LEMMA
        THEN ASSUME_TAC FUNPOW_COMP_LEMMA
        THEN ASM_REWRITE_TAC []
    ]
 );
 
-(* --------------------------------------------------------*)
-(* - Time-Consistency One-Step Theorems -------------------*)
-(* --------------------------------------------------------*)
+(*--------------------------------------------------------
+  - Time-Consistency One-Step Theorems -------------------
+  --------------------------------------------------------*)
 
 val SPLIT_ITER_LEMMA = prove(
-  `!G init next Imm dur t a. IMAP G init next ==>
-    (G (SUC t) a = (FUNPOW next 1 (G t a)))`,
+  `!f init next dur. IMAP f init next ==>
+    (!t a. f (SUC t) a = (FUNPOW next 1 (f t a)))`,
   REPEAT STRIP_TAC
     THEN IMP_RES_TAC STATE_FUNPOW_LEMMA
-    THEN FULL_SIMP_TAC std_ss [FUNPOW_COMP_LEMMA,UIMM_def,ONE,
-                               ADD_CLAUSES,FUNPOW,FUNPOW_THM]
+    THEN FULL_SIMP_TAC bool_ss [FUNPOW_COMP_LEMMA,UIMMERSION_def,ONE,
+                                ADD_CLAUSES,FUNPOW,FUNPOW_THM]
 );
 
 val TC_ONE_STEP_THM = store_thm("TC_ONE_STEP_THM",
-  `!G init next. IMAP G init next ==>
-    (TCON G =
-      ((!a. init (G 0 a) = G 0 a) /\
-       (!a. init (G 1 a) = G 1 a)))`,
-  REPEAT STRIP_TAC
-    THEN IMP_RES_TAC TC_LEMMA
-    THEN NTAC 2 (POP_ASSUM (K ALL_TAC))
-    THEN POP_ASSUM (fn th => REWRITE_TAC [th])
-    THEN EQ_TAC  THENL [
-      RW_TAC std_ss [],
-      REPEAT STRIP_TAC
-        THEN Induct_on `t` THENL [
-          ASM_REWRITE_TAC [],
-          IMP_RES_TAC SPLIT_ITER_LEMMA
-            THEN POP_ASSUM (fn th => REWRITE_TAC [th])
-            THEN POP_ASSUM (fn th => ONCE_REWRITE_TAC [SYM th])
-            THEN IMP_RES_TAC STATE_FUNPOW_LEMMA
-            THEN POP_ASSUM (fn th => REWRITE_TAC [GSYM th])
-            THEN ASM_REWRITE_TAC []
-        ]
+  `!f. TCON f =
+         IS_IMAP f /\
+         (!a. f 0 (f 0 a) = f 0 a) /\
+         (!a. f 0 (f 1 a) = f 1 a)`,
+  RW_TAC bool_ss [TC_THM]
+    THEN EQ_TAC THEN REPEAT STRIP_TAC
+    THEN ASM_REWRITE_TAC []
+    THEN FULL_SIMP_TAC bool_ss [IS_IMAP_def]
+    THEN Induct_on `t`
+    THENL [
+      ASM_REWRITE_TAC [],
+      IMP_RES_TAC SPLIT_ITER_LEMMA
+        THEN POP_ASSUM (fn th => REWRITE_TAC [th])
+        THEN PAT_ASSUM `f 0 (f t a) = f t a` (fn th => ONCE_REWRITE_TAC [SYM th])
+        THEN IMP_RES_TAC IMAP_INIT
+        THEN IMP_RES_TAC STATE_FUNPOW_LEMMA
+        THEN POP_ASSUM (fn th => ASM_REWRITE_TAC [GSYM th])
+        THEN POP_ASSUM (fn th => ASM_REWRITE_TAC [SYM th])
     ]
 );
 
 val SPLIT_ITER_LEMMA' = prove(
-  `!G init next imm dur t a. (IMAP G init next /\ UIMM imm G dur) ==>
-    ((G (dur (init (G (imm a t) a)) + imm a t) a) =
-    (FUNPOW next (imm (G (imm a t) a) 1) (G (imm a t) a)))`,
+  `!f init next imm dur. IMAP f init next /\ UIMMERSION imm f dur ==>
+    (!t a. f (dur (f 0 (f (imm a t) a)) + imm a t) a =
+           FUNPOW next (imm (f (imm a t) a) 1) (f (imm a t) a))`,
   REPEAT STRIP_TAC
     THEN IMP_RES_TAC STATE_FUNPOW_LEMMA
-    THEN FULL_SIMP_TAC std_ss [FUNPOW_COMP_LEMMA,UIMM_def,ONE,
-                               ADD_CLAUSES,FUNPOW,FUNPOW_THM]
+    THEN FULL_SIMP_TAC bool_ss [FUNPOW_COMP_LEMMA,UIMMERSION_def,ONE,
+                                ADD_CLAUSES,FUNPOW,FUNPOW_THM]
 );
 
-val TC_IMM_ONE_STEP_THM = store_thm("TC_IMM_ONE_STEP_THM",
-  `!G init next imm dur. (IMAP G init next /\ UIMM imm G dur) ==>
-    (TCON_IMM G imm =
-      ((!a. init (G (imm a 0) a) = G (imm a 0) a) /\
-       (!a. init (G (imm a 1) a) = G (imm a 1) a)))`,
+val TC_IMMERSION_ONE_STEP_THM = store_thm("TC_IMMERSION_ONE_STEP_THM",
+  `!f imm . IS_IMAP f /\ UNIFORM imm f ==>
+    (TCON_IMMERSION f imm =
+       (!a. f 0 (f (imm a 0) a) = f (imm a 0) a) /\
+       (!a. f 0 (f (imm a 1) a) = f (imm a 1) a))`,
   REPEAT STRIP_TAC
-    THEN IMP_RES_TAC UIMM_IS_IMM_LEMMA
-    THEN IMP_RES_TAC TC_IMM_LEMMA
-    THEN NTAC 2 (POP_ASSUM (K ALL_TAC))
-    THEN ASM_REWRITE_TAC []
-    THEN EQ_TAC 
-    THEN STRIP_TAC THENL [
-        ASM_REWRITE_TAC [],
-        Induct_on `t` THENL [
-          ASM_REWRITE_TAC [],
-          GEN_TAC
-            THEN PAT_ASSUM `UIMM Imm G dur`
-                 (fn th => REWRITE_TAC [REWRITE_RULE [UIMM_def] th] THEN
-                 ASSUME_TAC th)
-            THEN PAT_ASSUM `!a. init (G (Imm a t) a) = G (Imm a t) a`
-                 (fn th => (ONCE_REWRITE_TAC [GSYM th] THEN
-                 ASSUME_TAC th))
-            THEN IMP_RES_TAC SPLIT_ITER_LEMMA'
-            THEN POP_ASSUM (fn th => REWRITE_TAC [th])
-            THEN POP_ASSUM (fn th => (ONCE_REWRITE_TAC [GSYM th] THEN
-                 ASSUME_TAC th))
-            THEN IMP_RES_TAC STATE_FUNPOW_LEMMA
-            THEN POP_ASSUM (fn th => REWRITE_TAC [GSYM th])
-            THEN POP_ASSUM (fn th => ONCE_REWRITE_TAC [th])
-            THEN ASM_REWRITE_TAC []
-        ]
+    THEN IMP_RES_TAC UNIFORM_IMP_IMMERSION
+    THEN EQ_TAC THEN STRIP_TAC
+    THEN ASM_SIMP_TAC bool_ss [TC_IMMERSION_LEMMA,TC_IMMERSION_LEMMA2]
+    THEN Induct
+    THENL [
+      ASM_REWRITE_TAC [],
+      GEN_TAC THEN FULL_SIMP_TAC bool_ss [UNIFORM_def,IS_IMAP_def]
+        THEN PAT_ASSUM `UIMMERSION imm f dur`
+             (fn th => REWRITE_TAC [REWRITE_RULE [UIMMERSION_def] th] THEN
+             ASSUME_TAC th)
+        THEN PAT_ASSUM `!a. f 0 (f (imm a t) a) = f (imm a t) a`
+             (fn th => (ONCE_REWRITE_TAC [GSYM th] THEN ASSUME_TAC th))
+        THEN IMP_RES_TAC SPLIT_ITER_LEMMA'
+        THEN POP_ASSUM (fn th => REWRITE_TAC [th])
+        THEN POP_ASSUM (fn th => (ONCE_REWRITE_TAC [GSYM th] THEN
+             ASSUME_TAC th))
+        THEN IMP_RES_TAC STATE_FUNPOW_LEMMA2
+        THEN POP_ASSUM (fn th => REWRITE_TAC [GSYM th])
+        THEN ASM_REWRITE_TAC []
     ]
 );
 
-(* --------------------------------------------------------*)
-(* - Correctnes One-Step Theorems -------------------------*)
-(* --------------------------------------------------------*)
+(*--------------------------------------------------------
+  - Correctnes One-Step Theorems -------------------------
+  --------------------------------------------------------*)
 
 val ONE_STEP_LEMMA = prove(
-  `!G init next imm dur t a. (IMAP G init next /\ UIMM imm G dur /\
-  TCON_IMM G imm) ==>
-  (imm a (SUC t) = (imm (G (imm a t) a) 1 + imm a t))`,
+  `!f imm dur.
+     UNIFORM imm f /\ TCON_IMMERSION f imm ==>
+     (!t a. imm a (SUC t) = (imm (f (imm a t) a) 1 + imm a t))`,
   REPEAT STRIP_TAC
-   THEN IMP_RES_TAC UIMM_IS_IMM_LEMMA
-   THEN IMP_RES_TAC TC_IMM_LEMMA
-   THEN FULL_SIMP_TAC std_ss [UIMM_def,ONE,ADD_CLAUSES,IMAP_def]
+   THEN IMP_RES_TAC UNIFORM_IMP_IMMERSION
+   THEN IMP_RES_TAC TC_IMMERSION_LEMMA
+   THEN FULL_SIMP_TAC bool_ss [UNIFORM_def,UIMMERSION_def,ONE,ADD_CLAUSES]
 );
 
 val ONE_STEP_THM = store_thm("ONE_STEP_THM",
-  `!spec impl initf nextf initg nextg imm dur psi.
-    (UIMM imm impl dur /\ ONTO_INIT psi initf initg /\
-     IMAP spec initf nextf /\
-     IMAP impl initg nextg /\
-     TCON spec /\ TCON_IMM impl imm) ==>
-    (CORRECT spec impl imm psi =
-    (!a. spec 0 (psi a) = psi (impl (imm a 0) a)) /\
-    (!a. spec 1 (psi a) = psi (impl (imm a 1) a)))`,
-  RW_TAC std_ss [CORRECT_def,TCON_def]
-    THEN IMP_RES_TAC ONE_STEP_LEMMA
-    THEN NTAC 2 (POP_ASSUM (K ALL_TAC))
-    THEN RULE_ASSUM_TAC (REWRITE_RULE [IMAP_def,GSYM FUN_EQ_THM])
-    THEN EQ_TAC THENL [
-      RW_TAC std_ss [],
-      REPEAT STRIP_TAC THENL [
-        IMP_RES_TAC UIMM_IS_IMM_LEMMA,
-        ASM_REWRITE_TAC [],
-        Induct_on `t` THENL [
-          ASM_REWRITE_TAC [],
-          PAT_ASSUM `!t a. imm a (SUC t) = imm (impl (imm a t) a) 1 + imm a t`
-                 (fn th => REWRITE_TAC [th])
-            THEN PAT_ASSUM `TCON_IMM impl imm`
-                 (fn th => REWRITE_TAC [REWRITE_RULE [TCON_IMM_def] th])
-            THEN PAT_ASSUM `!a. spec 1 (psi a) = psi (impl (imm a 1) a)`
-                 (fn th => REWRITE_TAC [ONE,GSYM th])
-            THEN POP_ASSUM (fn th => REWRITE_TAC [GSYM th])
-            THEN PAT_ASSUM `!t1 t2 a. spec (t1 + t2) a = spec t1 (spec t2 a)`
-                 (fn th => REWRITE_TAC [SYM (num_CONV ``1``),GSYM (SPECL [`SUC 0`,`t`] th)])
-            THEN SIMP_TAC arith_ss [ADD1]
-        ]
-      ]
-    ]
-);
-      
-(* --------------------------------------------------------*)
-
-val ONE_STEP_SUP_LEMMA = prove(
-  `!G init next Imm1 Imm2 dur1 dur2 r a.
-  AUIMM Imm1 Imm2 G dur1 dur2 /\ IMAP G init next /\
-  TCON_IMM G Imm2 ==>
-  (Imm1 a (SUC r) = (Imm1 (G (Imm2 a r) a) 1 + Imm1 a r))`,
+  `!spec impl imm abs.
+      (UNIFORM imm impl /\
+       TCON spec /\
+       TCON_IMMERSION impl imm) ==>
+      (CORRECT spec impl imm abs =
+        DATA_ABSTRACTION abs (spec 0) (impl 0) /\
+        (!a. spec 0 (abs a) = abs (impl (imm a 0) a)) /\
+         !a. spec 1 (abs a) = abs (impl (imm a 1) a))`,
   REPEAT STRIP_TAC
-   THEN IMP_RES_TAC AUIMM_IS_IMM_LEMMA
-   THEN IMP_RES_TAC TC_IMM_LEMMA
-   THEN FULL_SIMP_TAC std_ss [AUIMM_def,UIMM_def,ONE,ADD_CLAUSES,IMAP_def]
-);
-
-val ONE_STEP_SUP_THM = store_thm("ONE_STEP_SUP_THM",
-  `!spec impl initf nextf initg nextg imm1 imm2 dur1 dur2 psi.
-    (AUIMM imm1 imm2 impl dur1 dur2 /\
-     ONTO_INIT psi initf initg /\
-     IMAP spec initf nextf /\
-     IMAP impl initg nextg /\
-     TCON spec /\ TCON_IMM impl imm2) ==>
-    (CORRECT_SUP spec impl imm1 imm2 psi =
-    (!a. spec (imm1 a 0) (psi a) = psi (impl (imm2 a 0) a)) /\
-    (!a. spec (imm1 a 1) (psi a) = psi (impl (imm2 a 1) a)))`,
-  RW_TAC std_ss [CORRECT_SUP_def,TCON_def]
-    THEN PAT_ASSUM `IMAP spec initf nextf`
-         (fn th => ASSUME_TAC (CONJ th (CONJUNCT1 (REWRITE_RULE [IMAP_def,GSYM FUN_EQ_THM] th))))
-    THEN PAT_ASSUM `IMAP impl initg nextg`
-         (fn th => ASSUME_TAC (CONJ th (CONJUNCT1 (REWRITE_RULE [IMAP_def,GSYM FUN_EQ_THM] th))))
-    THEN EQ_TAC THENL [
-      RW_TAC std_ss  [],
-      REPEAT STRIP_TAC THENL [
-        IMP_RES_TAC AUIMM_IS_IMM_LEMMA,
-        IMP_RES_TAC AUIMM_IS_IMM_LEMMA,
-        ASM_REWRITE_TAC [],
-        Induct_on `r` THENL [
-          ASM_REWRITE_TAC [],
-          FULL_SIMP_TAC std_ss []
-           THEN IMP_RES_TAC ONE_STEP_SUP_LEMMA
-           THEN POP_ASSUM (K ALL_TAC)
-           THEN POP_ASSUM (fn th => REWRITE_TAC [th])
-           THEN `UIMM imm2 impl dur2` by IMP_RES_TAC AUIMM_def
-           THEN `!t a. imm2 a (SUC t) = imm2 (impl (imm2 a t) a) 1 + imm2 a t`
-             by IMP_RES_TAC ONE_STEP_LEMMA
-           THEN REWRITE_TAC [ONE]
-           THEN POP_ASSUM (fn th => REWRITE_TAC [th])
-           THEN PAT_ASSUM `TCON_IMM impl imm2`
-                (fn th => REWRITE_TAC [REWRITE_RULE [TCON_IMM_def] th])
-           THEN PAT_ASSUM `!a. spec (imm1 a 1) (psi a) = psi (impl (imm2 a 1) a)`
+    THEN IMP_RES_TAC ONE_STEP_LEMMA
+    THEN EQ_TAC
+    THEN RW_TAC bool_ss [CORRECT_def]
+    THENL [
+       IMP_RES_TAC UNIFORM_IMP_IMMERSION,
+       Induct_on `t` THENL [
+         ASM_REWRITE_TAC [],
+         PAT_ASSUM `!t a. imm a (SUC t) = imm (impl (imm a t) a) 1 + imm a t`
+           (fn th => REWRITE_TAC [th])
+           THEN PAT_ASSUM `TCON_IMMERSION impl imm`
+                (fn th => REWRITE_TAC [REWRITE_RULE [TCON_IMMERSION_def] th])
+           THEN PAT_ASSUM `!a. spec 1 (abs a) = abs (impl (imm a 1) a)`
                 (fn th => REWRITE_TAC [ONE,GSYM th])
-           THEN POP_ASSUM (K ALL_TAC)
            THEN POP_ASSUM (fn th => REWRITE_TAC [GSYM th])
-           THEN ASM_REWRITE_TAC []
-        ]
-      ]
+           THEN RULE_ASSUM_TAC (REWRITE_RULE [TCON_def])
+           THEN PAT_ASSUM `!t1 t2 a. spec (t1 + t2) a = spec t1 (spec t2 a)`
+                (fn th => REWRITE_TAC [SYM ONE,GSYM (SPECL [`SUC 0`,`t`] th)])
+           THEN SIMP_TAC arith_ss [ADD1]
+       ]
     ]
 );
 
 (* --------------------------------------------------------*)
 
 val IMAP_COMP = store_thm("IMAP_COMP",
-  `!G init next t a. IMAP G init next ==>
-     (G t a = if t = 0 then init a else next (G (t-1) a))`,
-   RW_TAC arith_ss [IMAP_def]
+  `!f init next. IMAP f init next ==>
+     (!t a. f t a = if t = 0 then init a else next (f (t-1) a))`,
+   REPEAT STRIP_TAC THEN FULL_SIMP_TAC bool_ss [IMAP_def]
+    THEN RW_TAC bool_ss []
     THEN RULE_ASSUM_TAC (REWRITE_RULE [NOT_ZERO_LT_ZERO])
     THEN IMP_RES_TAC LESS_ADD_1
     THEN RW_TAC arith_ss [GSYM ADD1]
 );
 
-val UIMM_COMP = prove(
-  `!Imm G dur t a. UIMM Imm G dur ==>
-     (Imm a t = if t = 0
-                then 0
-                else dur (G (Imm a (t-1)) a) + Imm a (t-1))`,
-   RW_TAC arith_ss [UIMM_def]
-    THEN RULE_ASSUM_TAC (REWRITE_RULE [NOT_ZERO_LT_ZERO])
-    THEN IMP_RES_TAC LESS_ADD_1
-    THEN RW_TAC arith_ss [GSYM ADD1]
-);
-
+(* --------------------------------------------------------*)
 (* --------------------------------------------------------*)
 
 val _ = export_theory();
